Restore working PropT for now

src/coq/Utils/PropT.v
@@ -64,7 +64,7 @@ Section ITreeMisc.
         : forall j1 j2, RI1 j1 j2 -> eutt (sum_rel RI2 RR) (body1 j1) (body2 j2))
     : forall (i1 : I1) (i2 : I2) (RI_i : RI1 i1 i2),
       @eutt E _ _ RR (ITree.iter body1 i1) (ITree.iter body2 i2).
-  Proof.
+  Proof using.
     einit. ecofix CIH. intros.
     specialize (eutt_body i1 i2 RI_i).
     do 2 rewrite unfold_iter.
@@ -78,7 +78,7 @@ Section ITreeMisc.
     @Proper ((A -> itree F (A + B)) -> A -> itree F B)
             ((R1 ==> eutt (sum_rel R2 S)) ==> R1 ==> (eutt S))
             (iter (C := ktree F)).
-  Proof.
+  Proof using.
     do 3 red;
     intros body1 body2 EQ_BODY x y Hxy. red in EQ_BODY.
     eapply eutt_iter''; eauto.
@@ -86,7 +86,7 @@ Section ITreeMisc.
 
   Lemma tau_eutt_RR_l : forall E R (RR : relation R) (HRR: Reflexive RR) (HRT: Transitive RR) (t s : itree E R),
       eutt RR (Tau t) s <-> eutt RR t s.
-  Proof.
+  Proof using.
     intros.
     split; intros H.
     - eapply transitivity. 2 : { apply H. }
@@ -96,14 +96,14 @@ Section ITreeMisc.
 
   Lemma tau_eqit_RR_l : forall E R (RR : relation R) (HRR: Reflexive RR) (HRT: Transitive RR) (t s : itree E R),
       eqit RR true false t s -> eqit RR true false (Tau t) s.
-  Proof.
+  Proof using.
     intros.
     red. pstep. econstructor. auto. punfold H.
   Qed.
 
   Lemma tau_eutt_RR_r : forall E R (RR : relation R) (HRR: Reflexive RR) (HRT: Transitive RR) (t s : itree E R),
       eutt RR t (Tau s) <-> eutt RR t s.
-  Proof.
+  Proof using.
     intros.
     split; intros H.
     - eapply transitivity. apply H.
@@ -113,7 +113,7 @@ Section ITreeMisc.
 
   Lemma eutt_flip : forall E R (RR : relation R) (t1 t2 : itree E R),
       eutt RR t1 t2 -> eutt (flip RR) t2 t1.
-  Proof.
+  Proof using.
     intros E R RR.
     einit.
     ecofix CIH.
@@ -152,14 +152,14 @@ Section PropMonad.
     fun PA PA' =>
       (forall x y, x ≈ y -> (PA x <-> PA' y)).
   
-  (* #[global] Polymorphic Instance Eq1_PropT {E} : Eq1 (PropT E) :=
-    fun a PA PA' =>
-      (forall x y, x ≈ y -> (PA x <-> PA' y)) /\
-      eutt_closed PA /\ eutt_closed PA'. *)
-
   #[global] Polymorphic Instance Eq1_PropT {E} : Eq1 (PropT E) :=
     fun a PA PA' =>
-      (forall x, (PA x <-> PA' x)).
+      (forall x y, x ≈ y -> (PA x <-> PA' y)) /\
+      eutt_closed PA /\ eutt_closed PA'.
+
+  (* #[global] Polymorphic Instance Eq1_PropT {E} : Eq1 (PropT E) :=
+    fun a PA PA' =>
+      (forall x, (PA x <-> PA' x)). *)
 
   #[global] Instance Functor_Prop {E}
     : Functor (PropT E) :=
@@ -167,6 +167,7 @@ Section PropMonad.
 
   Inductive Returns {E} {A: Type} (a: A) : itree E A -> Prop :=
   | ReturnsRet: forall t, t ≈ Ret a -> Returns a t
+  | ReturnsTau: forall t u, t ≈ Tau u -> Returns a u -> Returns a t
   | ReturnsVis: forall {X} (e: E X) (x: X) t k, t ≈ Vis e k -> Returns a (k x) -> Returns a t
   .
   Hint Constructors Returns: core.
@@ -203,7 +204,7 @@ Section PropMonad.
     (* Example bind_constraint {E: Type -> Type} (e: (E nat)):
     let single_propT := (fun t => t ≈ (Vis e (@ret (itree E) _ nat))) in
     eq1 (bind_PropT _ _ single_propT (@ret (PropT E) _ nat)) single_propT.
-    Proof.
+    Proof using.
       cbn.
       split; intros.
       unfold bind_PropT in H.
@@ -253,27 +254,13 @@ Section PropMonad.
 
   Lemma bind_PropT_bind_PropT' {E}:
     forall A B PA K (tb : itree E B), bind_PropT A B PA K tb <-> bind_PropT' A B PA K tb.
-  Proof.
+  Proof using.
     intros. split.
     intros.
     - red. red in H.
       destruct H as (ta & ka & HPA & Heq & HR).
       exists ta. split; auto.
-      left.  
-      eexists (fun a => tb).
-      split; cycle 1.
-
-      assert (eutt eq ta (ret ka)).
-      admit.
-      rewrite H.
-      rewrite bind_ret_l.
-      reflexivity.
-
-      
-      intros.
-
-      auto.
-      exists tb. split; auto.
+      left.  exists ka. split; auto.
     - intros.
       red. red in H.
       destruct H as  (ta & EQ1 & [(k & KA & EQ2) | HX]).
@@ -288,7 +275,7 @@ Section PropMonad.
 
 
   Lemma Returns_ret_inv_ : forall {E} A (a b : A) (t : itree E A), t ≈ (Ret b) -> Returns a t -> a = b.
-  Proof.
+  Proof using.
     intros E A a b t eq H.
     revert b eq.
     induction H; intros; subst.
@@ -298,7 +285,7 @@ Section PropMonad.
   Qed.
 
   Lemma Returns_ret_inv :  forall {E} A (a b : A), Returns a ((ret b) : itree E A) -> a = b.
-  Proof.
+  Proof using.
     intros.
     eapply Returns_ret_inv_. reflexivity. cbn in H. apply H.
   Qed.
@@ -317,7 +304,7 @@ Section PropMonad.
                 ITree.bind (step' i) (@iter_cont I E R step') ≈ r /\
                 (forall j, step j (step' j))).
 
-  (* This exists in the stdlib as [ProofIrrelevance.inj_pair2], but we reprove
+  (* This exists in the stdlib as [Proof using.rrelevance.inj_pair2], but we reprove
    it to not depend on proof irrelevance (we use axiom [JMeq.JMeq_eq] instead).
    The itree library now avoids as much as possible using this axiom, we may want
    to see if it's possible to do so here.
@@ -325,7 +312,7 @@ Section PropMonad.
   Lemma inj_pair2 :
     forall (U : Type) (P : U -> Type) (p : U) (x y : P p),
       existT P p x = existT P p y -> x = y.
-  Proof.
+  Proof using.
     intros. apply JMeq.JMeq_eq.
     refine (
         match H in _ = w return JMeq.JMeq x (projT2 w) with
@@ -337,7 +324,7 @@ Section PropMonad.
         (t : itree E T)  (k1: T -> itree E R) (k2 : T -> itree E S) :
     (eutt RS  (ITree.bind t k1) (ITree.bind t k2)) ->
     (forall r, Returns r t -> eutt RS (k1 r) (k2 r)).
-  Proof.
+  Proof using.
     intros EQIT r HRET.
     revert R S RS k1 k2 EQIT.
     induction HRET; intros.
@@ -363,7 +350,7 @@ Section PropMonad.
   Qed.
 
   #[global] Instance Returns_eutt {E A} a: Proper (eutt eq ==> iff) (@Returns E A a).
-  Proof.
+  Proof using.
     repeat intro; split; intros HRet.
     - revert y H. induction HRet; intros.
       constructor; rewrite <- H, H0; reflexivity.
@@ -378,14 +365,14 @@ Section PropMonad.
   Qed.
 
   Lemma Returns_Vis_sub :  forall {E} {R} X (e : E X) (k : X -> itree E R) u x, Returns u (k x) -> Returns u (Vis e k).
-  Proof.
+  Proof using.
     intros.
     eapply ReturnsVis. reflexivity. apply H.
   Qed.
 
   Lemma eutt_Returns_ : forall {E} {R} (RR : R -> Prop) (ta : itree E R)
      (IN: forall (a : R), Returns a ta -> RR a), eutt (fun u1 u2 => u1 = u2 /\ RR u1) ta ta.
-  Proof.
+  Proof using.
     intros E R.
     ginit.
     gcofix CIH; intros.
@@ -402,7 +389,7 @@ Section PropMonad.
   Qed.
 
   Lemma eutt_Returns : forall E R (ta : itree E R), eutt (fun u1 u2 => u1 = u2 /\ Returns u1 ta) ta ta.
-  Proof.
+  Proof using.
     intros.
     apply eutt_Returns_. auto.
   Qed.
@@ -428,7 +415,7 @@ Section PropMonad.
           (CMP: compose (eqitC RS b1 b2) vclo <3= compose vclo (eqitC RS b1 b2))
           (ID: id <3= vclo):
       eqit_Returns_bind_clo b1 b2 <3= gupaco2 (eqit_ RS b1 b2 vclo) (eqitC RS b1 b2).
-    Proof.
+    Proof using.
       gcofix CIH. intros. destruct PR.
       guclo eqit_clo_trans.
       econstructor; auto_ctrans_eq; try (rewrite (itree_eta (x <- _;; _ x)), unfold_bind; reflexivity).
@@ -480,7 +467,7 @@ Section PropMonad.
       eqit eq b1 b2 t1 t2 ->
       (forall r, Returns r t1 -> eqit eq b1 b2 (k1 r) (k2 r)) ->
     @eqit E _ _ eq b1 b2 (ITree.bind t1 k1) (ITree.bind t2 k2).
-  Proof.
+  Proof using.
   intros. ginit. guclo (@eqit_Returns_clo_bind E R R eq). unfold eqit in *.
   econstructor; eauto with paco.
   Qed.
@@ -490,19 +477,19 @@ Section PropMonad.
       eqit eq b1 b2 t1 t2 ->
       (forall r, Returns r t1 -> eqit RS b1 b2 (k1 r) (k2 r)) ->
     @eqit E _ _ RS b1 b2 (ITree.bind t1 k1) (ITree.bind t2 k2).
-  Proof.
+  Proof using.
   intros. ginit. guclo (@eqit_Returns_clo_bind E R S RS). unfold eqit in *.
   econstructor; eauto with paco.
   Qed.
 
   Lemma eutt_ret_vis_abs: forall {X Y E} {RR : relation X} (x: X) (e: E Y) k, eutt RR (Ret x) (Vis e k) -> False.
-  Proof.
+  Proof using.
     intros.
     punfold H; inv H.
   Qed.
 
   Lemma Returns_Ret_ : forall E A (a x : A) (t:itree E A), t ≈ Ret x -> Returns a t -> x = a.
-  Proof.
+  Proof using.
     intros E A a x t eq H.
     induction H.
     - rewrite eq in H. eapply eqit_inv in H. apply H.
@@ -511,7 +498,7 @@ Section PropMonad.
   Qed.
 
   Lemma Returns_Ret :  forall E A (a x : A), Returns a ((Ret x) : itree E A) -> x = a.
-  Proof.
+  Proof using.
     intros.  eapply Returns_Ret_. 2: eassumption. reflexivity.
   Qed.
 
@@ -519,7 +506,7 @@ Section PropMonad.
     (HM: Returns a ma)
     (HK: Returns b (k a)),
       Returns b (bind ma k).
-  Proof.
+  Proof using.
     intros.
     revert B b k HK.
     induction HM; intros.
@@ -532,7 +519,7 @@ Section PropMonad.
       Returns b u ->
       u ≈ (bind t k) ->
       exists a, Returns a t /\ Returns b (k a).
-  Proof.
+  Proof using.
     intros E A B u t k b HR eq.
     revert A t k eq.
     induction HR; intros.
@@ -566,7 +553,7 @@ Section PropMonad.
   Lemma Returns_bind_inversion : forall {E A B} (t : itree E A) (k : A -> itree E B) b,
       Returns b (bind t k) ->
       exists a, Returns a t /\ Returns b (k a).
-  Proof.
+  Proof using.
     intros.
     eapply Returns_bind_inversion_. apply H. reflexivity.
   Qed.
@@ -575,7 +562,7 @@ Section PropMonad.
       Returns b u ->
       u ≈ (Vis e k) ->
       exists a, Returns b (k a).
-  Proof.
+  Proof using.
     intros E A B u e k b HR eq.
     revert A e k eq.
     induction HR; intros.
@@ -603,7 +590,7 @@ Section PropMonad.
   Lemma Returns_vis_inversion : forall {E A B} (e : E A) (k : A -> itree E B) b,
       Returns b (Vis e k) ->
       exists a, Returns b (k a).
-  Proof.
+  Proof using.
     intros.
     eapply Returns_vis_inversion_. apply H. reflexivity.
   Qed.
@@ -612,7 +599,7 @@ Section PropMonad.
 
   Lemma Returns_divergent {E A}:
     (forall (ta : itree E A), not (exists a, Returns a ta) -> divergent ta).
-  Proof.
+  Proof using.
     intros. red. intros. red in H.
     unfold bind, Monad_itree.
     generalize dependent ta. pcofix CIH. cbn. pstep. unfold eqit_.
@@ -657,7 +644,7 @@ Section IterLaws.
            (f >>> case_ (g x0 a1) inr_)
        ⩯
        f >>> case_ (iter (C := Kleisli (itree E)) (bif := sum) ((g x0 a1) >>> (case_ f inr_))) (id_ _).
-  Proof.
+  Proof using.
     intros. rewrite iter_dinatural. reflexivity.
   Qed.
 
@@ -679,7 +666,7 @@ Section IterLaws.
                     | inl i0 => ret (inl (i0, S k))
                     | inr r0 => ret (inr r0)
                     end)) (a1, 1).
-  Proof.
+  Proof using.
     intros a b m x0 a1.
     pose proof (iter_succ_dinatural x0 a1) as H0.
     specialize (H0 (a1, 0)).
@@ -736,7 +723,7 @@ Section MonadLaws.
       eutt_closed PA /\ eutt_closed PA'. *)
 
   (* Lemma Eq1_PropT'_Eq1_PropT : forall E a PA PA', @Eq1_PropT E a PA PA' -> Eq1_PropT' a PA PA'.
-  Proof.
+  Proof using.
     intros.
     red.
     red in H.
@@ -751,7 +738,7 @@ Section MonadLaws.
 
    #[global] Instance ret_PropT_Proper {E R} :
      Proper (eq ==> eutt eq ==> iff) (@ret (PropT E) _ R).
-   Proof.
+   Proof using.
    repeat red.
    intros.
    split;  cbn; intros; red; red; subst.
@@ -764,25 +751,29 @@ Section MonadLaws.
   Lemma ret_bind: forall {E} (a b : Type) (f : a -> PropT E b) (x : a),
       eutt_closed (f x) ->
       eq1 (bind (ret x) f) (f x).
-  Proof.
+  Proof using.
     intros.
-    (* split; [| split]. *)
-    split.
-    - intros eqtt'.
+    split; [| split].
+    -  intros t t' eq; split; intros eqtt'.
       * cbn in *.
         repeat red in eqtt'.
         destruct eqtt' as (ta & k & EQ1 & EQ2 & KA).
-        + unfold bind, Monad_itree in EQ2. rewrite EQ1, Eqit.bind_ret_l in EQ2.
+        + unfold bind, Monad_itree in EQ2. rewrite EQ1, Eqit.bind_ret_l, eq in EQ2.
           eapply H; [apply EQ2 | apply KA].
           constructor 1; eauto.
-      
-    - intros HX.
-      * repeat red in H.
-        specialize (H)
-        destruct H.
+      * cbn.
+        eexists (Ret x), (fun _ => t); split; [reflexivity|]; split.
+         + unfold bind, Monad_itree. rewrite Eqit.bind_ret_l; reflexivity.
+         + intros.
+           apply Returns_Ret in H0. subst. red in H. rewrite eq.
+           assumption.
+    - intros t t' EQ; cbn; split; intros HX.
+      * destruct HX as (ta & k & EQ1 & EQ2 & KA).
         exists (Ret x), (fun _ => t); split; [reflexivity |]; split.
-        --  unfold bind, Monad_itree. rewrite Eqit.bind_ret_l. symmetry. assumption.
-        --
+         + unfold bind, Monad_itree. 
+          rewrite Eqit.bind_ret_l.
+          symmetry. assumption.
+        + 
           intros ? RET; inv RET.
           2: { rewrite tau_eutt in H0. rewrite <- H0 in H1. apply Returns_Ret in H1. subst.
                red in H. rewrite EQ2. rewrite EQ1.
@@ -793,7 +784,7 @@ Section MonadLaws.
           eapply H. rewrite EQ1 in EQ2.
           unfold bind, Monad_itree in EQ2.
              rewrite Eqit.bind_ret_l in EQ2. apply EQ2.
-             apply KA; rewrite EQ1; constructor; reflexivity.
+             apply KA; rewrite EQ1; constructor; reflexivity. 
 
       * destruct HX as (ta & k & EQ1 & EQ2 & KA).
         exists (Ret x), (fun _ => t); split; [reflexivity |]; split.
@@ -818,7 +809,7 @@ Section MonadLaws.
 
    #[global] Instance bind_PropT_Proper {E} {A B} :
      Proper (eq1 ==> (eq ==> eq1) ==> eutt eq ==> iff) (@bind_PropT E A B).
-   Proof.
+   Proof using.
      repeat red; intros PA1 PA2 EQP K1 K2 EQK t1 t2 EQt; split; intros H.
      - destruct H as (ta & k & HA & eq & HK).
        red.
@@ -838,7 +829,7 @@ Section MonadLaws.
 
    #[global] Instance bind_Propt_Proper2 {E} {A B} (PA : PropT E A) (K : A -> PropT E B) :
      Proper (eutt eq ==> flip impl) (bind PA K).
-   Proof.
+   Proof using.
      repeat red.
      intros.
      repeat red in H0.
@@ -858,7 +849,7 @@ Section MonadLaws.
 
   Lemma agree_itree_Returns : forall E A B (ta : itree E A) (K : A -> PropT E B) (k : A -> itree E B),
       (forall a, Returns a ta -> K a (k a)) <-> (agrees_itree (fmap k ta) (fmap K ta)).
-  Proof.
+  Proof using.
     intros.
     split; intros.
     - cbn. red.
@@ -914,7 +905,7 @@ Section MonadLaws.
         (HRET : Returns a ma)
         (NEQ: ~((k1 a) ≈ (k2 a))) :
     not ((ITree.bind ma k1) ≈ (ITree.bind ma k2)).
-  Proof.
+  Proof using.
     intro HI.
     apply NEQ. clear NEQ.
     revert k1 k2 HI.
@@ -933,7 +924,7 @@ Section MonadLaws.
 
   Lemma not_Returns {E} {A B} : inhabited B ->
     forall (ta: itree E A), (exists tb, forall (k : A -> itree E B), tb ≈ bind ta k) -> forall (a:A), ~ Returns a ta.
-  Proof.
+  Proof using.
     intros IB ta HX a HRet; inversion IB; clear IB.
     revert HX.
     induction HRet; intros (tb & HK).
@@ -970,7 +961,7 @@ Section MonadLaws.
   Lemma bind_ret: forall {E} (A : Type) (PA : PropT E A),
       eutt_closed PA ->
       eq1 (bind PA (fun x => ret x)) PA.
-  Proof.
+  Proof using.
     intros.
     split; [| split].
     + intros t t' eq; split; intros eqtt'.
@@ -1007,7 +998,7 @@ Section MonadLaws.
     fun a b => a = b /\ Returns a ta.
 
   Lemma Symmteric_EQ_REL {E A} (ta : itree E A) : Symmetric (EQ_REL ta).
-  Proof.
+  Proof using.
     repeat red.
     intros a b (EQ & H).
     split.
@@ -1016,7 +1007,7 @@ Section MonadLaws.
   Qed.
 
   Lemma Transitive_EQ_REL {E A} (ta : itree E A) : Transitive (EQ_REL ta).
-  Proof.
+  Proof using.
     repeat red.
     intros a b c (EQ1 & H1) (EQ2 & H2).
     split.
@@ -1025,7 +1016,7 @@ Section MonadLaws.
   Qed.
 
   Instance EQ_REL_Proper {E A} : Proper (eutt eq ==> eq ==> eq ==> iff) (@EQ_REL E A).
-  Proof.
+  Proof using.
     repeat red.
     intros. subst.
     split; intros; unfold EQ_REL in *.
@@ -1041,7 +1032,7 @@ Section MonadLaws.
 
   Instance eutt_EQ_REL_Proper {E} {A} :
     Proper (eq_relation ==> eutt eq ==> @eutt E A A eq ==> iff) (eutt).
-  Proof.
+  Proof using.
     repeat red.
     intros; split; intros.
     -  rewrite <- H0. rewrite <- H1.
@@ -1056,7 +1047,7 @@ Section MonadLaws.
   Lemma eutt_EQ_REL_Reflexive_ {E} {A} (ta : itree E A) :
     forall R, (EQ_REL ta) <2= R ->
     eutt R ta ta.
-  Proof.
+  Proof using.
     revert ta.
     ginit. gcofix CIH. intros ta HEQ.
     gstep. red.
@@ -1078,7 +1069,7 @@ Section MonadLaws.
   Qed.
 
   Lemma eutt_EQ_REL_Reflexive {E} {A} (ta : itree E A) : eutt (EQ_REL ta) ta ta.
-  Proof.
+  Proof using.
     apply eutt_EQ_REL_Reflexive_.
     auto.
   Qed.
@@ -1103,7 +1094,7 @@ Lemma bind_bind_Prop: forall {E}
                    (KCP : Proper (eq ==> eq1) KC)
                    (t : itree E C),
       (bind (bind PA KB) KC) t -> (bind PA (fun a => bind (KB a) KC)) t.
-  Proof.
+  Proof using.
     (* PA ~a> KB a ~b> KC b *)
     intros E A B C PA KB KC PQOK KBP KCP t eqtt'.
         red in eqtt'.
@@ -1143,7 +1134,7 @@ Module BIND_BIND_COUNTEREXAMPLE.
                                else bind (trigger Pick) (fun (x:bool)  => if x then ret false else ITree.spin)).
 
   Lemma bind_right_assoc : bind PA (fun a => bind (KB a) KC) t.
-  Proof.
+  Proof using.
     repeat red.
     exists (trigger Pick).
     exists (fun (b:bool) => if b
@@ -1172,7 +1163,7 @@ Module BIND_BIND_COUNTEREXAMPLE.
   Qed.
 
   Lemma not_bind_left_assoc : ~ (bind (bind PA KB) KC t).
-  Proof.
+  Proof using.
     intro H.
     repeat red in H.
     destruct H as (ta & k & HB & HEQ & HRET).
@@ -1213,7 +1204,7 @@ Qed.
 
 Lemma bind_bind_counterexample:
     exists t, bind PA (fun a => bind (KB a) KC) t /\ ~ (bind (bind PA KB) KC t).
-Proof.
+Proof using.
   exists t.
   split.
   apply bind_right_assoc.
